Proofs/Stuttering.thy
@@ -5,7 +5,7 @@ theory Stuttering
     Semantics.IRStepObj
 begin
 
-inductive stutter:: "IRGraph \<Rightarrow> MapState \<Rightarrow> Params \<Rightarrow> FieldRefHeap \<Rightarrow> ID \<Rightarrow> ID \<Rightarrow> bool" ("_ _ _ _ \<turnstile> _ \<leadsto> _" 55)
+inductive stutter:: "IRGraph \<Rightarrow> MapState \<Rightarrow> Params \<Rightarrow> RefFieldHeap \<Rightarrow> ID \<Rightarrow> ID \<Rightarrow> bool" ("_ _ _ _ \<turnstile> _ \<leadsto> _" 55)
   for g m p h where
 
   StutterStep:
